Split into multiple .v files

Proofs.v
@@ -1,3 +1,4 @@
+From LeapSecurity Require Export Core.
 Require Import Coq.Sets.Ensembles.
 Require Import Coq.Sets.Finite_sets.
 Require Import Coq.Sets.Constructive_sets.
@@ -7,59 +8,20 @@ Require Import Coq.Logic.Classical.
 Require Import Coq.Logic.Classical_Prop.
 Require Import Coq.Arith.PeanoNat.
 Require Import Coq.Lists.List.
+
 Import ListNotations.
-Module ListEnsemble.
-  Definition in_set := Ensembles.In.
-  Definition add_set := Ensembles.Add.
-End ListEnsemble.
 Import ListEnsemble.
 
-Inductive difficulty : Type := Hard | Easy.
-Inductive strength : Type := Strong | Weak.
-Inductive safety : Type := Safe | Dangerous.
-
-Definition text := nat.
-Definition key := text.
-Definition salt := text.
-Definition password := text.
-Definition ciphertext := text.
-Definition textSet := Ensemble text.
-Definition beq_text := Nat.eqb.
-Record key_pair := {pub: key; pr: key}.
-
-Parameter PWD: password.
-Parameter Salt: salt.
-Parameter MEK: key.
-Parameter MK DK: key_pair.
-
-Parameter TextRelated: text -> text -> Prop.
-Definition UnrelatedSet l t := forall h,
-  (in_set text l h) -> ~(TextRelated t h).
-
-Fixpoint as_set (l: list text) : textSet :=
-  match l with
-  | [] => Empty_set text
-  | x :: xs => add_set text (as_set xs) x
-  end.
-
-Parameter Guess:
-  textSet -> text -> difficulty.
-Axiom nilGuess:
-  forall t, Guess (as_set []) t = Hard.
-Axiom incHardGuess: forall t h l,
-  (Guess l t = Hard) /\ ~(TextRelated t h) ->
-  (Guess (add_set text l h) t = Hard).
-
-Lemma unrelatedGuess: forall uset t,
+Lemma unrelatedSafe: forall uset t,
   Finite text uset -> UnrelatedSet uset t ->
-  Guess uset t = Hard.
+  Safe uset t.
 Proof.
   intros ll t l.
   induction l as [| l' l'f H m H0].
   - intro H1.
-    apply nilGuess.
+    apply nilSafe.
   - intro H1.
-    apply incHardGuess.
+    apply incSafe.
     split.
     apply H.
     intros h H2.
@@ -72,14 +34,14 @@ Proof.
     auto.
 Qed.
 
-Lemma unionTwoUnrelatedHardGuess:
+Lemma unionTwoUnrelatedSafe:
   forall s1 s2 t, Finite text s1 ->
   Finite text s2 ->
   UnrelatedSet s1 t /\ UnrelatedSet s2 t ->
-  Guess (Union text s1 s2) t = Hard.
+  Safe (Union text s1 s2) t.
 Proof.
   intros ll1 ll2 t l1 l2 H.
-  apply unrelatedGuess.
+  apply unrelatedSafe.
   apply Union_preserves_Finite.
   auto. auto.
   intros h H3.
@@ -91,11 +53,11 @@ Proof.
   auto. auto. auto.
 Qed.
 
-Lemma unionUnrelatedHardGuess:
+Lemma unionUnrelatedSafe:
   forall s s' t, Finite text s ->
   Finite text s' -> UnrelatedSet s' t ->
-  Guess s t = Hard ->
-  Guess (Union text s s') t = Hard.
+  Safe s t ->
+  Safe (Union text s s') t.
 Proof.
   intros ll1 ll2 t l1 l2 H H0.
   induction l2 as [| l' l'f H1 m H2].
@@ -106,7 +68,7 @@ Proof.
     trivial.
   - specialize (Union_add text ll1 l' m) as H3.
     rewrite <- H3.
-    apply incHardGuess.
+    apply incSafe.
     split.
     apply H1.
     assert (H4: UnrelatedSet (add_set text l' m) t -> UnrelatedSet l' t).
@@ -129,56 +91,13 @@ Proof.
     auto.
 Qed.
 
-Parameter Rare: text -> Prop.
-Axiom invRare: forall f t,
-  Rare (f t) -> Rare t.
-
-Parameter E_Sym D_Sym:
-  key -> text -> text.
-Axiom symEnDe:
-  forall k t, D_Sym k (E_Sym k t) = t.
-Axiom symDeEn:
-  forall k t, E_Sym k (D_Sym k t) = t.
-Axiom symTextSafety: forall k t,
-  Guess (as_set [E_Sym k t]) t = Hard.
-
-Axiom asymKeySafety: forall kp,
-  Guess (as_set [pr kp]) (pub kp) = Hard.
-
-Parameter E_Asym D_Asym:
-  key -> text -> text.
-Axiom asymEnDe: forall kp t,
-  D_Asym (pr kp) (E_Asym (pub kp) t) = t.
-Axiom asymDeEn: forall kp t,
-  E_Asym (pub kp) (D_Asym (pr kp) t) = t.
-
-Parameter Hash: text -> text.
-Axiom rareConflictHash: forall t1 t2,
-  Hash t1 = Hash t2 ->
-  (Rare t2 /\
-  Guess (as_set [Hash t1]) t2 = Hard).
 Lemma onewayHash: forall t,
-  Guess (as_set [Hash t]) t = Hard.
+  Safe (as_set [Hash t]) t.
 Proof.
   intro t.
   apply rareConflictHash.
   trivial.
 Qed.
-
-Parameter Kdf: password -> salt -> key.
-
-Definition KEK := Kdf PWD Salt.
-Definition KEK_MEK := E_Sym KEK MEK.
-Definition H_MEK := Hash MEK.
-Inductive auth_option :=
-  | ASome (mek : key)
-  | AFail.
-
-Definition Auth (PWD_t:password) :=
-  let KEK_t := Kdf PWD_t Salt in
-  let MEK_t := D_Sym KEK_t KEK_MEK in
-  if (beq_text (Hash MEK_t) H_MEK)
-    then ASome MEK_t else AFail.
 
 (*
   A correct password is able to unlock the MEK
@@ -233,7 +152,7 @@ Proof.
   assert (H7: Rare (D_Sym (Kdf p Salt) KEK_MEK)).
   {
     assert (H8: Rare (D_Sym (Kdf p Salt) KEK_MEK) /\
-      Guess (as_set [Hash MEK]) (D_Sym (Kdf p Salt) KEK_MEK) = Hard).
+      Safe (as_set [Hash MEK]) (D_Sym (Kdf p Salt) KEK_MEK) ).
     {
       auto.
     }
@@ -297,7 +216,7 @@ Proof.
       assert (HD: Rare (D_Sym (Kdf p Salt) KEK_MEK)).
       {
         assert (HP: Rare (D_Sym (Kdf p Salt) KEK_MEK) /\
-          Guess (as_set [Hash MEK]) (D_Sym (Kdf p Salt) KEK_MEK) = Hard).
+          Safe (as_set [Hash MEK]) (D_Sym (Kdf p Salt) KEK_MEK) ).
         {
           auto.
         }
@@ -314,34 +233,6 @@ Proof.
       contradiction.
   - auto.
 Qed.
-
-Parameter Sign: key -> text -> text.
-Parameter Verify:
-  key -> text -> text -> bool.
-Axiom signCorrect: forall kp t sig,
-  sig = Sign (pr kp) t \/ Rare sig <->
-  Verify (pub kp) t sig = true.
-
-Definition MSign t := Sign (pr MK) t.
-Definition MVerify t sig :=
-  Verify (pub MK) t sig.
-Definition SIG := MSign (pub DK).
-
-Inductive wrap_option :=
-  | WSome (e_mek : text)
-  | WFail.
-Record wrapped := {mek: key; nonce: nat}.
-Parameter Conc: wrapped -> text.
-Parameter Splt: text -> wrapped.
-Axiom SplitConcatenation:
-  forall w, w = Splt (Conc w).
-
-Definition Wrap mek k sig n :=
-  if (MVerify k sig)
-    then let w := {|mek := mek;
-                  nonce := n|} in
-    WSome (E_Asym k (Conc w))
-    else WFail.
 
 Lemma correctWrap:
   forall mek k sig n,
@@ -382,16 +273,6 @@ Proof.
     inversion H2.
 Qed.
 
-Inductive unwrap_option :=
-  | USome (mek : text)
-  | UFail.
-Definition Unwrap w n:=
-  let uw :=
-    Splt (D_Asym (pr DK) w) in
-  if (beq_text (nonce uw) n)
-    then USome (mek uw)
-    else UFail.
-
 Lemma correctUnwrap:
   forall w n,
   nonce w = n ->
@@ -431,9 +312,9 @@ Qed.
 
 (*
 
-(* TODO: Hard instead of ~ *)
+(* TODO:  instead of ~ *)
 Axiom signAuthority:
-  forall s k, Guess s k = Hard ->
+  forall s k, Safe s k  ->
   forall kp t sig, pr kp = k ->
   ~(Verify (pub kp) t sig).
 Axiom signIntegrity:.
@@ -442,7 +323,7 @@ Axiom goodKdf: forall p s p',
   let kek := (Kdf p s) in
   kek = Kdf p' s ->
   (Rare p' /\
-  Guess (as_set [s;kek]) p' = Hard).
+  Safe (as_set [s;kek]) p' ).
 Lemma rareConflictKdf: forall p s p',
   p <> p' /\ Kdf p s = Kdf p' s ->
   Rare p'.
@@ -453,9 +334,9 @@ Proof.
   destruct H3 as [H4 H5].
   auto. auto.
 Qed.
-Theorem saltyKdf: forall p s, Guess (as_set [p]) (Kdf p s) = Hard.
-Axiom onewayKdf: forall p s, Guess (as_set [Kdf p s]) p = Hard.
-Axiom incEasyGuess: forall t h l, (Guess l t <> Hard) -> (Guess (add_set text l h) t <> Hard).
+Theorem saltyKdf: forall p s, Safe (as_set [p]) (Kdf p s).
+Axiom onewayKdf: forall p s, Safe (as_set [Kdf p s]) p.
+Axiom incEasySafe: forall t h l, (Safe l t <> ) -> (Safe (add_set text l h) t <> ).
 
 Parameter TextStrength: text -> strength.
 Parameter WeakSet: textSet.
