Core.v
@@ -1,0 +1,35 @@
+From LeapSecurity Require Export Definitions.
+
+Parameter PWD: password.
+Parameter Salt: salt.
+Parameter MEK: key.
+Parameter MK DK: key_pair.
+
+Definition KEK := Kdf PWD Salt.
+Definition KEK_MEK := E_Sym KEK MEK.
+Definition H_MEK := Hash MEK.
+
+Definition MSign t := Sign (pr MK) t.
+Definition MVerify t sig :=
+  Verify (pub MK) t sig.
+Definition SIG := MSign (pub DK).
+
+Definition Auth (PWD_t:password) :=
+  let KEK_t := Kdf PWD_t Salt in
+  let MEK_t := D_Sym KEK_t KEK_MEK in
+  if (beq_text (Hash MEK_t) H_MEK)
+    then ASome MEK_t else AFail.
+
+Definition Wrap mek k sig n :=
+  if (MVerify k sig)
+    then let w := {|mek := mek;
+                  nonce := n|} in
+    WSome (E_Asym k (Conc w))
+    else WFail.
+
+Definition Unwrap w n:=
+  let uw :=
+    Splt (D_Asym (pr DK) w) in
+  if (beq_text (nonce uw) n)
+    then USome (mek uw)
+    else UFail.
