Definitions.v
@@ -1,0 +1,81 @@
+Require Import Coq.Sets.Ensembles.
+Require Import Coq.Lists.List.
+Import ListNotations.
+
+Module ListEnsemble.
+  Definition in_set := Ensembles.In.
+  Definition add_set := Ensembles.Add.
+End ListEnsemble.
+Import ListEnsemble.
+
+Definition text := nat.
+Definition key := text.
+Definition salt := text.
+Definition password := text.
+Definition ciphertext := text.
+Definition textSet := Ensemble text.
+Definition beq_text := Nat.eqb.
+
+Record key_pair := {pub: key; pr: key}.
+Record wrapped := {mek: key; nonce: nat}.
+
+Inductive auth_option :=
+  | ASome (mek : key)
+  | AFail.
+Inductive wrap_option :=
+  | WSome (e_mek : text)
+  | WFail.
+Inductive unwrap_option :=
+  | USome (mek : text)
+  | UFail.
+
+Parameter TextRelated: text -> text -> Prop.
+Definition UnrelatedSet l t := forall h,
+  (in_set text l h) -> ~(TextRelated t h).
+
+Fixpoint as_set (l: list text) : textSet :=
+  match l with
+  | [] => Empty_set text
+  | x :: xs => add_set text (as_set xs) x
+  end.
+
+Parameter Safe: textSet -> text -> Prop.
+Parameter Rare: text -> Prop.
+Parameter E_Sym D_Sym:
+  key -> text -> text.
+Parameter E_Asym D_Asym:
+  key -> text -> text.
+Parameter Hash: text -> text.
+Parameter Kdf: password -> salt -> key.
+Parameter Sign: key -> text -> text.
+Parameter Verify:
+  key -> text -> text -> bool.
+Parameter Conc: wrapped -> text.
+Parameter Splt: text -> wrapped.
+
+Axiom nilSafe: forall t, Safe (as_set []) t.
+Axiom incSafe: forall t h l,
+  (Safe l t) /\ ~(TextRelated t h) ->
+  (Safe (add_set text l h) t).
+Axiom invRare: forall f t,
+  Rare (f t) -> Rare t.
+Axiom symEnDe:
+  forall k t, D_Sym k (E_Sym k t) = t.
+Axiom symDeEn:
+  forall k t, E_Sym k (D_Sym k t) = t.
+Axiom symTextSafety: forall k t,
+  Safe (as_set [E_Sym k t]) t .
+Axiom asymKeySafety: forall kp,
+  Safe (as_set [pr kp]) (pub kp) .
+Axiom asymEnDe: forall kp t,
+  D_Asym (pr kp) (E_Asym (pub kp) t) = t.
+Axiom asymDeEn: forall kp t,
+  E_Asym (pub kp) (D_Asym (pr kp) t) = t.
+Axiom rareConflictHash: forall t1 t2,
+  Hash t1 = Hash t2 ->
+  (Rare t2 /\ Safe (as_set [Hash t1]) t2).
+Axiom signCorrect: forall kp t sig,
+  sig = Sign (pr kp) t \/ Rare sig <->
+  Verify (pub kp) t sig = true.
+Axiom SplitConcatenation:
+  forall w, w = Splt (Conc w).
